finish imp to asm

theories/imp_to_asm.v
@@ -169,7 +169,7 @@ Definition imp_to_asm_ret (rs rsold : gmap string Z) (v : val) : Prop.
 (* R0 contain representation of v *)
 Admitted.
 
-Definition imp_to_asm_itree_from_env (ins : gset Z) (fns : gset string) (f2i : gmap string Z) : itree (moduleE (imp_event + asm_event) ()) () :=
+Definition imp_to_asm_itree_from_env (ins : gset Z) (fns : gset string) (f2i : gmap string Z) : itree (moduleE (imp_event + asm_event) (list (bool * Z * gmap string Z))) () :=
   pc ← TExist Z;;;
   rs ← TExist _;;;
   TVis (inr (EARecvJump pc rs));;;;
@@ -186,21 +186,30 @@ Definition imp_to_asm_itree_from_env (ins : gset Z) (fns : gset string) (f2i : g
     TAssume (f ∈ fns);;;;
     (* env proves it calls the right address *)
     TAssume (f2i !! f = Some pc);;;;
+    (* env proves that ret is not in invs *)
+    TAssume (ret ∉ ins);;;;
     (* env proves that rs corresponds to vs and ret  *)
     TAssume (imp_to_asm_args ret rs vs);;;;
+    (* track the registers and return address (false means ret belongs to env) *)
+    cs ← TGet;;; TPut ((false, ret, rs)::cs);;;;
     TVis (inl (EIRecvCall f vs))
   else
     (* env chooses return value *)
     v ← TAll _;;;
     (* env chooses old registers *)
     rsold ← TAll _;;;
-    (* TODO: get rsold from call stack *)
+    (* env chooses rest of cs *)
+    cs' ← TAll _;;;
+    (* get registers from stack (true means pc belongs to the program) *)
+    cs ← TGet;;;
+    TAssume (cs = (true, pc, rsold)::cs');;;;
+    TPut cs';;;;
     (* env proves that rs is updated correctly *)
     TAssume (imp_to_asm_ret rs rsold v);;;;
     TVis (inl (EIRecvReturn v))
 .
 
-Definition imp_to_asm_itree_to_env (ins : gset Z) (fns : gset string) (f2i : gmap string Z) : itree (moduleE (imp_event + asm_event) ()) () :=
+Definition imp_to_asm_itree_to_env (ins : gset Z) (fns : gset string) (f2i : gmap string Z) : itree (moduleE (imp_event + asm_event) (list (bool * Z * gmap string Z))) () :=
   pc ← TExist Z;;;
   rs ← TExist _;;;
   (* program chooses whether it returns or makes a function call *)
@@ -216,8 +225,12 @@ Definition imp_to_asm_itree_to_env (ins : gset Z) (fns : gset string) (f2i : gma
     TAssert (f ∉ fns);;;;
     (* program proves that the address is correct *)
     TAssert (f2i !! f = Some pc);;;;
+    (* program proves that ret is in invs *)
+    TAssert (ret ∈ ins);;;;
     (* program proves that rs corresponds to vs and ret  *)
     TAssert (imp_to_asm_args ret rs vs);;;;
+    (* track the registers and return address (true means ret belongs to program) *)
+    cs ← TGet;;; TPut ((true, ret, rs)::cs);;;;
     TVis (inl (EICall f vs));;;;
     TVis (inr (EAJump pc rs))
   else
@@ -225,59 +238,108 @@ Definition imp_to_asm_itree_to_env (ins : gset Z) (fns : gset string) (f2i : gma
     v ← TExist _;;;
     (* program chooses old registers *)
     rsold ← TExist _;;;
-    (* TODO: get rsold from call stack *)
+    (* program chooses rest of cs *)
+    cs' ← TExist _;;;
+    (* get registers from stack (false means pc belongs to the env) *)
+    cs ← TGet;;;
+    TAssert (cs = (false, pc, rsold)::cs');;;;
+    TPut cs';;;;
     (* env proves that rs is updated correctly *)
     TAssert (imp_to_asm_ret rs rsold v);;;;
     TVis (inl (EIReturn v));;;;
     TVis (inr (EAJump pc rs)).
 
-Definition imp_to_asm_itree (ins : gset Z) (fns : gset string) (f2i : gmap string Z) : itree (moduleE (imp_event + asm_event) ()) () :=
+Definition imp_to_asm_itree (ins : gset Z) (fns : gset string) (f2i : gmap string Z) : itree (moduleE (imp_event + asm_event) (list (bool * Z * gmap string Z))) () :=
   ITree.forever (imp_to_asm_itree_from_env ins fns f2i;;;; imp_to_asm_itree_to_env ins fns f2i).
 
 Definition imp_to_asm (m : module imp_event) : module asm_event :=
-  mod_seq_map m (mod_itree (imp_event + asm_event) ()).
+  mod_seq_map m (mod_itree (imp_event + asm_event) (list (bool * Z * gmap string Z))).
 
 Definition initial_imp_to_asm_state (m : module imp_event) (σ : m.(m_state)) (ins : gset Z) (fns : gset string) (f2i : gmap string Z) : (imp_to_asm m).(m_state) :=
-  (SPRight, σ, (imp_to_asm_itree ins fns f2i, ()), SMFilter).
+  (SPRight, σ, (imp_to_asm_itree ins fns f2i, []), SMFilter).
+
+Inductive imp_to_asm_combine_stacks (ins1 ins2 : gset Z) :
+  list (imp_prod_filter_enum * imp_prod_filter_enum) →
+  list (bool * Z * gmap string Z) → list (bool * Z * gmap string Z) → list (bool * Z * gmap string Z) →
+ Prop :=
+| IAC_nil :
+  imp_to_asm_combine_stacks ins1 ins2 [] [] [] []
+| IAC_NoneLeft ret rs ics cs cs1 cs2:
+  ret ∉ ins1 →
+  ret ∉ ins2 →
+  default IPFNone (fst <$> head ics) = IPFNone →
+  imp_to_asm_combine_stacks ins1 ins2 ics cs cs1 cs2 →
+  imp_to_asm_combine_stacks ins1 ins2 ((IPFLeft, IPFNone) :: ics) ((false, ret, rs) :: cs) ((false, ret, rs) :: cs1) cs2
+| IAC_NoneRight ret rs ics cs cs1 cs2:
+  ret ∉ ins1 →
+  ret ∉ ins2 →
+  default IPFNone (fst <$> head ics) = IPFNone →
+  imp_to_asm_combine_stacks ins1 ins2 ics cs cs1 cs2 →
+  imp_to_asm_combine_stacks ins1 ins2 ((IPFRight, IPFNone) :: ics) ((false, ret, rs) :: cs) cs1 ((false, ret, rs) :: cs2)
+| IAC_LeftRight ret rs ics cs cs1 cs2:
+  ret ∈ ins1 →
+  fst <$> head ics = Some IPFLeft →
+  imp_to_asm_combine_stacks ins1 ins2 ics cs cs1 cs2 →
+  imp_to_asm_combine_stacks ins1 ins2 ((IPFRight, IPFLeft) :: ics) cs ((true, ret, rs) :: cs1) ((false, ret, rs) :: cs2)
+| IAC_LeftNone ret rs ics cs cs1 cs2:
+  ret ∈ ins1 →
+  fst <$> head ics = Some IPFLeft →
+  imp_to_asm_combine_stacks ins1 ins2 ics cs cs1 cs2 →
+  imp_to_asm_combine_stacks ins1 ins2 ((IPFNone, IPFLeft) :: ics) ((true, ret, rs) :: cs) ((true, ret, rs) :: cs1) cs2
+| IAC_RightLeft ret rs ics cs cs1 cs2:
+  ret ∈ ins2 →
+  fst <$> head ics = Some IPFRight →
+  imp_to_asm_combine_stacks ins1 ins2 ics cs cs1 cs2 →
+  imp_to_asm_combine_stacks ins1 ins2 ((IPFLeft, IPFRight) :: ics) cs ((false, ret, rs) :: cs1) ((true, ret, rs) :: cs2)
+| IAC_RightNone ret rs ics cs cs1 cs2:
+  ret ∈ ins2 →
+  fst <$> head ics = Some IPFRight →
+  imp_to_asm_combine_stacks ins1 ins2 ics cs cs1 cs2 →
+  imp_to_asm_combine_stacks ins1 ins2 ((IPFNone, IPFRight) :: ics) ((true, ret, rs) :: cs) cs1 ((true, ret, rs) :: cs2)
+.
 
 Definition imp_to_asm_combine_inv (m1 m2 : module imp_event)
            (ins1 ins2 : gset Z) (fns1 fns2 : gset string) (f2i1 f2i2 : gmap string Z)
   (σ1 : (asm_prod ins1 ins2 (imp_to_asm m1) (imp_to_asm m2)).(m_state))
   (σ2 : (imp_to_asm (imp_prod fns1 fns2 m1 m2)).(m_state)) : Prop :=
-  let '(σpa, (σpi1, σi1, (t1, _), σf1), (σpi2, σi2, (t2, _), σf2), σfa) := σ1 in
-  let '(σps, (σpi, σs1, σs2, σf), (t, _), σfs) := σ2 in
+  let '(σpa, (σpi1, σi1, (t1, cs1), σf1), (σpi2, σi2, (t2, cs2), σf2), σfa) := σ1 in
+  let '(σps, (σpi, σs1, σs2, σf), (t, cs), σfs) := σ2 in
   let ins := (ins1 ∪ ins2) in
   let fns := (fns1 ∪ fns2) in
   let f2i := (f2i1 ∪ f2i2) in
+  ∃ ics,
   σi1 = σs1 ∧
   σi2 = σs2 ∧
-  ((∃ cs,
-      σfa = APFNone ∧
-      σpa = SPNone ∧ σfs = SMFilter ∧ σps = SPRight ∧ t = imp_to_asm_itree ins fns f2i
+  imp_to_asm_combine_stacks ins1 ins2 ics cs cs1 cs2 ∧
+  (( σfa = APFNone ∧ σpa = SPNone ∧ σfs = SMFilter ∧ σps = SPRight ∧ t = imp_to_asm_itree ins fns f2i
       ∧ t1 = imp_to_asm_itree ins1 fns1 f2i1 ∧ t2 = imp_to_asm_itree ins2 fns2 f2i2
       ∧ σf1 = SMFilter ∧ σf2 = SMFilter ∧ σpi1 = SPRight ∧ σpi2 = SPRight
-      ∧ σpi = SPNone ∧ σf = IPFState IPFNone cs) ∨
-  (∃ cs,
-      ( (∃ f vs, σf = IPFState (IPFLeftRecvCall f vs) cs ∧ σf1 = SMProgRecv (EIRecvCall f vs))
-      ∨ (∃ v, σf = IPFState (IPFLeftRecvReturn v) cs ∧ σf1 = SMProgRecv (EIRecvReturn v))
-      ∨ σf = IPFState IPFLeft cs ∧ σf1 = SMProg)
+      ∧ σpi = SPNone ∧ σf = IPFState IPFNone ics
+      ∧ default IPFNone (fst <$> head ics) = IPFNone
+    ) ∨
+  (( (∃ f vs, σf = IPFState (IPFLeftRecvCall f vs) ics ∧ σf1 = SMProgRecv (EIRecvCall f vs))
+      ∨ (∃ v, σf = IPFState (IPFLeftRecvReturn v) ics ∧ σf1 = SMProgRecv (EIRecvReturn v))
+      ∨ σf = IPFState IPFLeft ics ∧ σf1 = SMProg)
       ∧ σfa = APFLeft ∧ σpa = SPLeft ∧ σfs = SMProg ∧ σps = SPLeft
       ∧ t = (imp_to_asm_itree_to_env ins fns f2i;;;; imp_to_asm_itree ins fns f2i)
       ∧ t1 = (imp_to_asm_itree_to_env ins1 fns1 f2i1;;;; (imp_to_asm_itree ins1 fns1 f2i1))
       ∧ t2 = imp_to_asm_itree ins2 fns2 f2i2
       ∧ σf2 = SMFilter ∧ σpi1 = SPLeft ∧ σpi2 = SPRight
-      ∧ σpi = SPLeft) ∨
-  (∃ cs,
-      ((∃ f vs, σf = IPFState (IPFRightRecvCall f vs) cs ∧ σf2 = SMProgRecv (EIRecvCall f vs))
-      ∨ (∃ v, σf = IPFState (IPFRightRecvReturn v) cs ∧ σf2 = SMProgRecv (EIRecvReturn v))
-      ∨ σf = IPFState IPFRight cs ∧ σf2 = SMProg)
+      ∧ σpi = SPLeft
+      ∧ fst <$> head ics = Some IPFLeft) ∨
+  (((∃ f vs, σf = IPFState (IPFRightRecvCall f vs) ics ∧ σf2 = SMProgRecv (EIRecvCall f vs))
+      ∨ (∃ v, σf = IPFState (IPFRightRecvReturn v) ics ∧ σf2 = SMProgRecv (EIRecvReturn v))
+      ∨ σf = IPFState IPFRight ics ∧ σf2 = SMProg)
       ∧ σfa = APFRight ∧ σpa = SPRight ∧ σfs = SMProg ∧ σps = SPLeft
       ∧ t = (imp_to_asm_itree_to_env ins fns f2i;;;; imp_to_asm_itree ins fns f2i)
       ∧ t1 = imp_to_asm_itree ins1 fns1 f2i1
       ∧ t2 = (imp_to_asm_itree_to_env ins2 fns2 f2i2;;;; (imp_to_asm_itree ins2 fns2 f2i2))
       ∧ σf1 = SMFilter ∧ σpi1 = SPRight ∧ σpi2 = SPLeft
-      ∧ σpi = SPRight)).
+      ∧ σpi = SPRight
+      ∧ fst <$> head ics = Some IPFRight)).
 Hint Constants Transparent : tstep.
+Ltac solve_imp_to_asm_combine_inv :=
+  eexists _; split_and!; [naive_solver..| try done; try by econs | naive_solver].
 
 Program Definition itree_step_forever_s EV S R (t : itree (moduleE EV S) R) s :=
   @eq_it_to_tstep_s EV S s (ITree.forever t) (t;;;;ITree.forever t) _.
@@ -314,9 +376,9 @@ Proof.
   move => Hdisji Hdisjf Hin1 Hin2 Hagree Ho1 Ho2.
   apply tsim_implies_trefines => /= n.
   unshelve apply: tsim_remember. { exact (λ _, imp_to_asm_combine_inv _ _ _ _ _ _ f2i1 f2i2). }
-  { naive_solver. } { done. }
-  move => /= {σ1 σ2} {}n Hloop [[[σpa [[[σpi1 σi1] [t1 []]] σf1]] [[[σpi2 σi2] [t2 []]] σf2]] σfa].
-  move => [[[σps [[[σpi σs1] σs2] σf]] [t []]] σfs] /= ?.
+  { solve_imp_to_asm_combine_inv. } { done. }
+  move => /= {σ1 σ2} {}n Hloop [[[σpa [[[σpi1 σi1] [t1 cs1]] σf1]] [[[σpi2 σi2] [t2 cs2]] σf2]] σfa].
+  move => [[[σps [[[σpi σs1] σs2] σf]] [t cs]] σfs] /= ?.
   destruct_all?; simplify_eq.
   - go_s. rewrite -/(imp_to_asm_itree _ _).
     go_s. go_s. go_i. invert_all asm_prod_filter.
@@ -327,7 +389,9 @@ Proof.
       go_i. go_i. go_i. go_i.
       invert_all asm_prod_filter.
       go_i. go_i. eexists b. go. destruct b.
-      * go_s. go_s. go_s. go_s. go_s. go_s. go_s. go_s. go_s. go_s. go_s. go_s. go_s. go_s.
+      * go_s. go_s. go_s. go_s. go_s. go_s. go_s. go_s. go_s. go_s. go_s. go_s.
+        go_s. go_s. go_s. go_s. go_s. go_s. go_s. go_s.
+        revert select (_ ∉ (_ ∪ _)) => /not_elem_of_union[??].
         revert select (_ ∈ (_ ∪ _)) => Hin. revert select ((_ ∪ _) !! _ = Some _) => Hf2i.
         move: Hin => /elem_of_union [Hf|Hf]. 2: {
           move: (Hf) => /Hin2[?[??]]. move: Hf2i => /lookup_union_Some_raw[?|[??]]; simplify_eq => //. naive_solver.
@@ -338,15 +402,18 @@ Proof.
         split; [done|].
         go_i. go_i. eexists _. go. go_i. go_i. eexists _. go. go_i. go_i. eexists _. go.
         go_i. go_i. split; [done|]. go. go_i. go_i. split; [done|]. go.
-        go_i. go_i. split; [done|]. go.
-        go_i. apply Hloop. naive_solver.
+        go_i. go_i. split; [done|]. go. go_i. go_i. split; [done|]. go. go_i. go_i.
+        go_i. go_i.
+        go_i. apply Hloop. solve_imp_to_asm_combine_inv.
         (* split_and! => //. right.  naive_solver. *)
-      * go_s. go_s. go_s. go_s. go_s. go_s. go_s. go_s.
-        have [cs' ?]: ∃ cs', cs = IPFLeft :: cs' by admit. subst.
+      * go_s. go_s. go_s. go_s. go_s. go_s. go_s. go_s. go_s. go_s. go_s. go_s. go_s. go_s. go_s. go_s.
+        revert select (imp_to_asm_combine_stacks _ _ _ _ _ _) => Hstack.
+        inversion Hstack; simplify_eq/= => //.
         eexists _, _, _. split; [apply IPFReturnExtToLeft|]. simpl. split; [done|].
         go_i. go_i. eexists _. go. go_i. go_i. eexists _. go.
+        go_i. go_i. eexists _. go. go_i. go_i. go_i. go_i. split; [done|]. go. go_i. go_i.
         go_i. go_i. split; [done|]. go.
-        go_i. apply Hloop. naive_solver.
+        go_i. apply Hloop. solve_imp_to_asm_combine_inv.
     + go_s. eexists _. go.
       go_s. go_s. eexists _. go. go_s. go_s. split; [done|]. go.
       go_s. go_s. rename x into b.
@@ -354,7 +421,9 @@ Proof.
       go_i. go_i. go_i. go_i.
       invert_all asm_prod_filter.
       go_i. go_i. eexists b. go. destruct b.
-      * go_s. go_s. go_s. go_s. go_s. go_s. go_s. go_s. go_s. go_s. go_s. go_s. go_s. go_s.
+      * go_s. go_s. go_s. go_s. go_s. go_s. go_s. go_s. go_s. go_s. go_s. go_s.
+        go_s. go_s. go_s. go_s. go_s. go_s. go_s. go_s.
+        revert select (_ ∉ (_ ∪ _)) => /not_elem_of_union[??].
         revert select (_ ∈ (_ ∪ _)) => Hin. revert select ((_ ∪ _) !! _ = Some _) => Hf2i.
         move: Hin => /elem_of_union [Hf|Hf]. 1: {
           move: (Hf) => /Hin1[?[??]]. move: Hf2i => /lookup_union_Some_raw[?|[??]]; simplify_eq => //.
@@ -365,47 +434,51 @@ Proof.
         split; [done|].
         go_i. go_i. eexists _. go. go_i. go_i. eexists _. go. go_i. go_i. eexists _.  go.
         go_i. go_i. split; [done|]. go. go_i. go_i. split; [done|]. go.
-        go_i. go_i. split; [done|]. go.
-        go_i. apply Hloop. naive_solver.
-      * go_s. go_s. go_s. go_s. go_s. go_s. go_s. go_s.
-        have [cs' ?]: ∃ cs', cs = IPFRight :: cs' by admit. subst.
+        go_i. go_i. split; [done|]. go. go_i. go_i. split; [done|]. go. go_i. go_i. go_i. go_i.
+        go_i. apply Hloop. solve_imp_to_asm_combine_inv.
+      * go_s. go_s. go_s. go_s. go_s. go_s. go_s. go_s. go_s. go_s. go_s. go_s. go_s. go_s. go_s. go_s.
+        revert select (imp_to_asm_combine_stacks _ _ _ _ _ _) => Hstack.
+        inversion Hstack; simplify_eq/= => //.
         eexists _, _, _. split; [apply IPFReturnExtToRight|]. simpl. split; [done|].
         go_i. go_i. eexists _. go. go_i. go_i. eexists _. go.
+        go_i. go_i. eexists _. go. go_i. go_i. go_i. go_i. split; [done|]. go. go_i. go_i.
         go_i. go_i. split; [done|]. go.
-        go_i. apply Hloop.  naive_solver.
+        go_i. apply Hloop. solve_imp_to_asm_combine_inv.
   - tstep_both.
     apply steps_impl_step_end => κ Pσ2. go. case_match; go.
     + tstep_s. eexists (Some (EIRecvCall f vs)), _. split; [done|]. eexists _, _. split; [econs|].
       apply: steps_spec_step_end; [done|] => ??. tend. eexists _. split; [done|].
-      apply: Hloop. naive_solver.
+      apply: Hloop. solve_imp_to_asm_combine_inv.
     + tstep_s. eexists None, _. split; [done|]. eexists _, _. split; [done|].
       apply: steps_spec_step_end; [done|] => ??. tend. eexists _. split; [done|].
-      apply: Hloop. naive_solver.
+      apply: Hloop. solve_imp_to_asm_combine_inv.
   - tstep_both.
     apply steps_impl_step_end => κ Pσ2. go. case_match; go.
     + tstep_s. eexists (Some (EIRecvReturn v)), _. split; [done|]. eexists _, _. split; [econs|].
       apply: steps_spec_step_end; [done|] => ??. tend. eexists _. split; [done|].
-      apply: Hloop. naive_solver.
+      apply: Hloop. solve_imp_to_asm_combine_inv.
     + tstep_s. eexists None, _. split; [done|]. eexists _, _. split; [done|].
       apply: steps_spec_step_end; [done|] => ??. tend. eexists _. split; [done|].
-      apply: Hloop. naive_solver.
+      apply: Hloop. solve_imp_to_asm_combine_inv.
   - tstep_both.
     apply steps_impl_step_end => κ Pσ2. go. destruct κ as [e|]; go.
     + tend. have [σ' Hσ'] := vis_no_all _ _ _ ltac:(done). eexists σ'. split; [naive_solver|].
       go_i. go_i. go_i. go_i. go_i. go_i. destruct x1.
       * go_i. go_i. go_i. go_i. go_i. go_i.
         go_i. go_i. go_i. go_i. go_i. go_i. go_i. go_i. go_i.
+        go_i. go_i. go_i. go_i. go_i. go_i.
         invert_all asm_prod_filter.
         -- go_i. go_i. go_i. go_i. go_i. go_i.
            go_i. go_i. invert_all asm_prod_filter.
            go_i. go_i. eexists true. go. go_i. go_i. eexists _. go.
            go_i. go_i. eexists _. go. go_i. go_i. eexists _. go.
            go_i. go_i. split; [ naive_solver|]. go. go_i. go_i. split; [naive_solver|]. go.
-           go_i. go_i. split; [done|]. go. go_i.
+           go_i. go_i. split; [by apply: Hdisji|]. go. go_i. go_i. split; [done|]. go. go_i. go_i. go_i.
+           go_i. go_i.
            go_s. eexists (Some _), _. split; [done|]. eexists _, _ => /=.
            split; [econs|]. { naive_solver. } { naive_solver. }
            apply: steps_spec_step_end; [done|] => ??.
-           apply: Hloop. naive_solver.
+           apply: Hloop. solve_imp_to_asm_combine_inv.
         -- go_s. eexists (Some _), _. split; [done|]. eexists _, _ => /=. split; [apply IPFCallLeftToExt|].
            { naive_solver. } { naive_solver. }
            apply: steps_spec_step_end; [done|] => ??.
@@ -414,65 +487,71 @@ Proof.
            go_s. go_s. eexists _. go. go_s. go_s. eexists _. go.
            go_s. go_s. split. { apply not_elem_of_union. naive_solver. }
            go. go_s. go_s. split. { apply lookup_union_Some_raw. naive_solver. }
-           go. go_s. go_s. split; [done|]. go. go_s. go_s. split; [done|]. go. go_s. split; [done|]. go.
-           apply: Hloop. naive_solver.
-      * go_i. go_i. go_i. go_i. go_i. go_i. go_i. go_i. go_i.
+           go. go_s. go_s. split; [apply elem_of_union; by left|]. go.
+           go_s. go_s. split; [done|]. go. go_s. go_s. go_s. go_s. go_s.
+           go_s. split; [done|]. go. go_s. split; [done|]. go.
+           apply: Hloop. solve_imp_to_asm_combine_inv.
+      * go_i. go_i. go_i. go_i. go_i. go_i. go_i. go_i. go_i. go_i. go_i. go_i. go_i. go_i. go_i. go_i. go_i.
         invert_all asm_prod_filter.
         -- go_i. go_i. go_i. go_i. go_i. go_i. go_i. go_i.
            invert_all asm_prod_filter.
-           have [cs' ?]: ∃ cs', cs = IPFRight :: cs' by admit. subst.
+           revert select (imp_to_asm_combine_stacks _ _ _ _ _ _) => Hstack.
+           inversion Hstack; simplify_eq/= => //.
            go_i. go_i. eexists false. go. go_i. go_i. eexists _. go.
-           go_i. go_i. eexists _. go. go_i. go_i. split; [done|]. go.
-           go_i.
+           go_i. go_i. eexists _. go. go_i. go_i. eexists _. go. go_i. go_i. go_i. go_i. split;[done|]. go.
+           go_i. go_i. go_i. go_i. split; [done|]. go. go_i.
            go_s. eexists (Some _), _. split; [done|]. eexists _, _ => /=.
            split; [apply IPFReturnLeftToRight|].
            apply: steps_spec_step_end; [done|] => ??.
-           apply: Hloop. naive_solver.
-        -- have [cs' ?]: ∃ cs', cs = IPFNone :: cs' by admit. subst.
+           apply: Hloop. solve_imp_to_asm_combine_inv.
+        -- revert select (imp_to_asm_combine_stacks _ _ _ _ _ _) => Hstack.
+           inversion Hstack; simplify_eq/= => //.
            go_s. eexists (Some _), _. split; [done|]. eexists _, _ => /=.
            split; [apply IPFReturnLeftToExt|].
            apply: steps_spec_step_end; [done|] => ??.
            go_s. go_s. eexists _. go. go_s. go_s. eexists _. go.
            go_s. go_s. eexists false. go. go_s. go_s. eexists _. go.
-           go_s. go_s. eexists _. go. go_s. go_s. split; [done|]. go.
+           go_s. go_s. eexists _. go. go_s. go_s. eexists _. go. go_s. go_s. go_s. go_s.
+           split; [done|]. go. go_s. go_s. go_s. go_s. split; [done|]. go.
            go_s. go_s. split; [done|]. go. go_s. split; [done|]. go.
-           apply: Hloop. naive_solver.
+           apply: Hloop. solve_imp_to_asm_combine_inv.
     + tstep_s. eexists None, _. split; [done|]. eexists _, _. split; [done|].
       apply: steps_spec_step_end; [done|] => ??. tend. eexists _. split; [done|].
-      apply: Hloop. naive_solver.
+      apply: Hloop. solve_imp_to_asm_combine_inv.
   - tstep_both.
     apply steps_impl_step_end => κ Pσ2. go. case_match; go.
     + tstep_s. eexists (Some (EIRecvCall f vs)), _. split; [done|]. eexists _, _. split; [econs|].
       apply: steps_spec_step_end; [done|] => ??. tend. eexists _. split; [done|].
-      apply: Hloop. naive_solver.
+      apply: Hloop. solve_imp_to_asm_combine_inv.
     + tstep_s. eexists None, _. split; [done|]. eexists _, _. split; [done|].
       apply: steps_spec_step_end; [done|] => ??. tend. eexists _. split; [done|].
-      apply: Hloop. naive_solver.
+      apply: Hloop. solve_imp_to_asm_combine_inv.
   - tstep_both.
     apply steps_impl_step_end => κ Pσ2. go. case_match; go.
     + tstep_s. eexists (Some (EIRecvReturn v)), _. split; [done|]. eexists _, _. split; [econs|].
       apply: steps_spec_step_end; [done|] => ??. tend. eexists _. split; [done|].
-      apply: Hloop. naive_solver.
+      apply: Hloop. solve_imp_to_asm_combine_inv.
     + tstep_s. eexists None, _. split; [done|]. eexists _, _. split; [done|].
       apply: steps_spec_step_end; [done|] => ??. tend. eexists _. split; [done|].
-      apply: Hloop. naive_solver.
+      apply: Hloop. solve_imp_to_asm_combine_inv.
   - tstep_both.
     apply steps_impl_step_end => κ Pσ2. go. destruct κ as [e|]; go.
     + tend. have [σ' Hσ'] := vis_no_all _ _ _ ltac:(done). eexists σ'. split; [naive_solver|].
       go_i. go_i. go_i. go_i. go_i. go_i. destruct x1.
-      * go_i. go_i. go_i. go_i. go_i. go_i.
-        go_i. go_i. go_i. go_i. go_i. go_i. go_i. go_i. go_i.
+      * go_i. go_i. go_i. go_i. go_i. go_i. go_i. go_i.
+        go_i. go_i. go_i. go_i. go_i. go_i. go_i. go_i. go_i. go_i. go_i. go_i. go_i.
         invert_all asm_prod_filter.
         -- go_i. go_i. go_i. go_i. go_i. go_i.
            go_i. go_i. invert_all asm_prod_filter.
            go_i. go_i. eexists true. go. go_i. go_i. eexists _. go.
            go_i. go_i. eexists _. go. go_i. go_i. eexists _. go.
            go_i. go_i. split; [ naive_solver|]. go. go_i. go_i. split; [naive_solver|]. go.
-           go_i. go_i. split; [done|]. go. go_i.
+           go_i. go_i. split. { move => ?. by apply: Hdisji. } go. go_i. go_i. split; [done|]. go.
+           go_i. go_i. go_i. go_i. go_i.
            go_s. eexists (Some _), _. split; [done|]. eexists _, _ => /=.
            split; [econs|]. { naive_solver. } { naive_solver. }
            apply: steps_spec_step_end; [done|] => ??.
-           apply: Hloop. naive_solver.
+           apply: Hloop. solve_imp_to_asm_combine_inv.
         -- go_s. eexists (Some _), _. split; [done|]. eexists _, _ => /=. split; [apply IPFCallRightToExt|].
            { naive_solver. } { naive_solver. }
            apply: steps_spec_step_end; [done|] => ??.
@@ -480,32 +559,38 @@ Proof.
            go_s. go_s. eexists true. go. go_s. go_s. eexists _. go.
            go_s. go_s. eexists _. go. go_s. go_s. eexists _. go.
            go_s. go_s. split. { apply not_elem_of_union. naive_solver. }
-           go. go_s. go_s. split.
-           { apply lookup_union_Some_raw. destruct (f2i1 !! x2) as [?|] eqn:?; naive_solver. }
-           go. go_s. go_s. split; [done|]. go. go_s. go_s. split; [done|]. go. go_s. split; [done|]. go.
-           apply: Hloop. naive_solver.
-      * go_i. go_i. go_i. go_i. go_i. go_i. go_i. go_i. go_i.
+           go. go_s. go_s. split. { apply lookup_union_Some_raw. destruct (f2i1 !! x2) eqn:?; naive_solver. }
+           go. go_s. go_s. split; [apply elem_of_union; by right|]. go. go_s. go_s. split; [done|]. go.
+           go_s. go_s. go_s. go_s. go_s.
+           go_s. split; [done|]. go. go_s. split; [done|]. go.
+           apply: Hloop. solve_imp_to_asm_combine_inv.
+      * go_i. go_i. go_i. go_i. go_i. go_i. go_i. go_i. go_i. go_i. go_i. go_i. go_i. go_i. go_i. go_i. go_i.
         invert_all asm_prod_filter.
         -- go_i. go_i. go_i. go_i. go_i. go_i. go_i. go_i.
            invert_all asm_prod_filter.
-           have [cs' ?]: ∃ cs', cs = IPFLeft :: cs' by admit. subst.
+           revert select (imp_to_asm_combine_stacks _ _ _ _ _ _) => Hstack.
+           inversion Hstack; simplify_eq/= => //.
            go_i. go_i. eexists false. go. go_i. go_i. eexists _. go.
-           go_i. go_i. eexists _. go. go_i. go_i. split; [done|]. go.
-           go_i.
+           go_i. go_i. eexists _. go. go_i. go_i. eexists _. go. go_i. go_i.
+           go_i. go_i. split;[done|]. go. go_i. go_i.
+           go_i. go_i. split; [done|]. go. go_i.
            go_s. eexists (Some _), _. split; [done|]. eexists _, _ => /=.
            split; [apply IPFReturnRightToLeft|].
            apply: steps_spec_step_end; [done|] => ??.
-           apply: Hloop. naive_solver.
-        -- have [cs' ?]: ∃ cs', cs = IPFNone :: cs' by admit. subst.
+           apply: Hloop. solve_imp_to_asm_combine_inv.
+        -- revert select (imp_to_asm_combine_stacks _ _ _ _ _ _) => Hstack.
+           inversion Hstack; simplify_eq/= => //.
            go_s. eexists (Some _), _. split; [done|]. eexists _, _ => /=.
            split; [apply IPFReturnRightToExt|].
            apply: steps_spec_step_end; [done|] => ??.
            go_s. go_s. eexists _. go. go_s. go_s. eexists _. go.
            go_s. go_s. eexists false. go. go_s. go_s. eexists _. go.
-           go_s. go_s. eexists _. go. go_s. go_s. split; [done|]. go.
+           go_s. go_s. eexists _. go. go_s. go_s. eexists _. go.
+           go_s. go_s. go_s. go_s. split; [done|]. go.
+           go_s. go_s. go_s. go_s. split; [done|]. go.
            go_s. go_s. split; [done|]. go. go_s. split; [done|]. go.
-           apply: Hloop. naive_solver.
+           apply: Hloop. solve_imp_to_asm_combine_inv.
     + tstep_s. eexists None, _. split; [done|]. eexists _, _. split; [done|].
       apply: steps_spec_step_end; [done|] => ??. tend. eexists _. split; [done|].
-      apply: Hloop. naive_solver.
-Abort.
+      apply: Hloop. solve_imp_to_asm_combine_inv.
+Qed.
